ulib/FStar.Tactics.Builtins.fsti
@@ -31,6 +31,9 @@ open FStar.VConfig
 (** Observe a sealed value. See Sealed.seal too. *)
 val unseal : #a:Type -> sealed a -> Tac a
 
+(** Resolve unification variable indirections at the top of the term. *)
+val compress : term -> Tac term
+
 (** [top_env] returns the environment where the tactic started running.
  * This works even if no goals are present. *)
 val top_env : unit -> Tac env
